Nerodia/Data/Py/Raw/Basic.lean
@@ -20,7 +20,7 @@ Returns whether two objects are identical (are the same pointer).
 This is equivalent to the Python {lit}`self is other`.
 -/
 @[extern "nerodia_py_object_dec_eq"]
-public def decEq (self other : Py.Raw) : Decidable (self = other) :=
+public def decEq (self other : @& Py.Raw) : Decidable (self = other) :=
   Classical.propDecidable _
 
 public instance : DecidableEq Py.Raw := decEq
